stlc/prop_nbe.v
@@ -13,6 +13,24 @@ Proof.
   apply eval_app_mutind; try sauto limit:50.
 Qed.
 
+Corollary eval_det : 
+  forall t ρ a1 a2, 
+  ⟦ t ⟧ ρ ↘ a1 -> 
+  ⟦ t ⟧ ρ ↘ a2 -> 
+  a1 = a2.
+Proof.
+  sauto use:app_eval_det.
+Qed.
+
+Corollary app_det : 
+  forall f a b1 b2, 
+  f ∙ a ↘ b1 -> 
+  f ∙ a ↘ b2 -> 
+  b1 = b2.
+Proof.
+  sauto use:app_eval_det.
+Qed.
+
 Lemma rne_rnf_det : 
   ( forall n e u1, Rⁿᵉ ⦇ n ⦈ e ↘ u1 -> forall u2, Rⁿᵉ ⦇ n ⦈ e ↘ u2 -> u1 = u2 ) /\ 
   ( forall n d v1, Rⁿᶠ ⦇ n ⦈ d ↘ v1 -> forall v2, Rⁿᶠ ⦇ n ⦈ d ↘ v2 -> v1 = v2 ).
